README.md
@@ -19,7 +19,7 @@ The Coq development of the source model (vRC11) and the IR model (PSir).
 - `src/model/Configuration.v`: Definition of a machine configuration and machine steps
 
 ### Soundness of mapping vRC11 to PSir (Theorem 4.2)
-- `Theorem pf_to_ir` in `src/pf2ir/PFtoIR.v`: Soundness of mapping vRC11 to PSir
+- `Theorem src_to_ir` in `src/src2ir/SrcToIR.v`: Soundness of mapping vRC11 to PSir
 
 ### Local DRF guarantees for vRC11
 - `Theorem local_drf_ra` in `src/ldrfra/LocalDRFRA.v`: Local DRF-RA guarantee
